Refactor: Move Network.Graph.Class into Network.Graph.Basic
Introduce Network.Graph.Class.Child

Hide 'scheme' in graph API behind functions on Graph.Class

Runtime/Network/Graph/Basic.lean
@@ -1,19 +1,68 @@
 import Runtime.Reaction
 import Runtime.Reactor
 
-namespace Network
-
-structure Graph where
+structure Network.Graph where
   classes : Type
   schemes : classes → (Reactor.Scheme classes)
   [decEqClasses : DecidableEq classes]
 
-attribute [instance] Graph.decEqClasses
+attribute [instance] Network.Graph.decEqClasses
 
-namespace Graph
+namespace Network.Graph
 
-abbrev interface (graph : Graph) («class» : graph.classes) :=
-  graph.schemes «class» |>.interface 
+def Class (graph : Graph) := graph.classes
 
-end Graph
-end Network
+namespace Class
+
+private def scheme (cls : Class graph) := graph.schemes cls
+
+def interface (cls : Class graph) := cls.scheme.interface
+
+abbrev timers (cls : Class graph) := cls.scheme.timers
+
+structure Child (cls : Class graph) where
+  id : cls.scheme.children
+  deriving DecidableEq
+
+def Child.class {cls : Class graph} (child : Child cls) : Class graph := 
+  cls.scheme.class child.id
+
+def subinterface (cls : Class graph) (kind : Reactor.InterfaceKind) :=
+  ⨄ fun child : Child cls => child.class.interface kind
+
+abbrev reactionInputScheme (cls : Class graph) :=
+  let localInputs := cls.interface .inputs
+  let nestedOutputs := cls.subinterface .outputs
+  localInputs ⊎ nestedOutputs
+
+abbrev reactionOutputScheme (cls : Class graph) :=
+  let localOutputs := cls.interface .outputs
+  let nestedInputs := cls.subinterface .inputs
+  localOutputs ⊎ nestedInputs
+
+abbrev reactionType (cls : Class graph) :=
+  Reaction 
+    cls.reactionInputScheme cls.reactionOutputScheme 
+    (cls.interface .actions) (cls.interface .state) (cls.interface .params) 
+    cls.scheme.timers
+
+structure Subport (cls : Class graph) (kind : Reactor.PortKind) where
+  child : Child cls
+  port : (child.class.interface kind).vars
+
+abbrev Subport.type (subport : Subport cls kind) : Type := 
+  (subport.child.class.interface kind).type subport.port
+
+-- TODO: The `eqTypeProof` is probably broken.
+macro "eqTypeProof" : tactic => `(intro input output; cases input <;> cases output <;> rename_i rtr₁ prt₁ rtr₂ prt₂ <;> cases rtr₁ <;> cases prt₁ <;> cases rtr₂ <;> cases prt₂ <;> simp)
+structure Connections (cls : Class graph) where 
+  source : (Subport cls .input) → Option (Subport cls .output)
+  eqType : (source input = some output) → (input.type = output.type) := by eqTypeProof
+
+def Connections.empty : Connections cls where
+  source _ := none
+  eqType := by simp
+
+end Class
+
+end Network.Graph
