Runtime/Network/Graph/Path/Basic.lean
@@ -1,10 +1,10 @@
-import Runtime.Network.Graph.Class
+import Runtime.Network.Graph.Basic
 
 namespace Network.Graph
 
 inductive Path (graph : Graph) : Class graph → Type _
   | nil : Path graph _
-  | cons {start : Class graph} (child : start.scheme.children) : Path graph (start.child child) → Path graph start
+  | cons {start : Class graph} (child : Class.Child start) : Path graph child.class → Path graph start
   deriving DecidableEq
 
 namespace Path
@@ -22,36 +22,16 @@ theorem cons_class : (Path.cons child subpath).class = subpath.class := rfl
 @[simp]
 theorem eq_class_iff_cons_eq_class : (path₁.class = path₂.class) ↔ (Path.cons child₁ path₁).class = (Path.cons child₂ path₂).class := ⟨id, id⟩
 
-abbrev scheme (path : Path graph start) := path.class.scheme
-
-@[simp]
-theorem nil_scheme : (nil : Path graph start).scheme = start.scheme := rfl
-
-@[simp]
-theorem cons_scheme : (Path.cons child subpath).scheme = subpath.scheme := rfl
-
-@[simp]
-theorem eq_scheme_iff_cons_eq_scheme : (path₁.scheme = path₂.scheme) ↔ (Path.cons child₁ path₁).scheme = (Path.cons child₂ path₂).scheme := ⟨id, id⟩
-
-abbrev reactionInputScheme (path : Graph.Path graph start) :=
-  path.class.reactionInputScheme
-
-abbrev reactionOutputScheme (path : Graph.Path graph start) :=
-  path.class.reactionOutputScheme 
-
-abbrev reactionType (path : Graph.Path graph start) :=
-  path.class.reactionType
-
-instance {path : Path graph start} {reaction : path.reactionType} : 
-  InjectiveCoe reaction.portSources path.reactionInputScheme.vars :=
+instance {path : Path graph start} {reaction : path.class.reactionType} : 
+  InjectiveCoe reaction.portSources path.class.reactionInputScheme.vars :=
   reaction.portSourcesInjCoe
 
-instance {path : Path graph start} {reaction : path.reactionType} : 
-  InjectiveCoe reaction.portEffects path.reactionOutputScheme.vars :=
+instance {path : Path graph start} {reaction : path.class.reactionType} : 
+  InjectiveCoe reaction.portEffects path.class.reactionOutputScheme.vars :=
   reaction.portEffectsInjCoe
 
-instance {path : Path graph start} {reaction : path.reactionType} : 
-  InjectiveCoe reaction.actionSources (path.scheme.interface .actions).vars :=
+instance {path : Path graph start} {reaction : path.class.reactionType} : 
+  InjectiveCoe reaction.actionSources (path.class.interface .actions).vars :=
   reaction.actionSourcesInjCoe
 
 end Path
