Runtime/Network/Graph.lean
@@ -1,3 +1,2 @@
 import Runtime.Network.Graph.Basic
-import Runtime.Network.Graph.Class
 import Runtime.Network.Graph.Path
